running clients for 1.3 + 1.2, more interop needed

src/tls/Handshake.fst
@@ -200,8 +200,11 @@ let processServerHello cfg ks log ri ch (ServerHello sh,_) =
            n_resume = false } in
 	   (match sh.sh_protocol_version, kex, next.ne_keyShare with
 	    | TLS_1p3, Kex_DHE, Some (gn,gyb) 
-	    | TLS_1p3, Kex_ECDHE, Some (gn,gyb) -> Correct (o_nego)
-            | _ -> Correct (o_nego))
+	    | TLS_1p3, Kex_ECDHE, Some (gn,gyb) -> 
+	      	   let lb = HandshakeLog.getHash log in
+	           let keys = KeySchedule.ks_client_13_1rtt ks o_nego.n_cipher_suite (gn, gyb) lb in
+	      	   Correct (o_nego,Some keys)
+            | _ -> Correct (o_nego,None))
 	| _ -> Error (AD_decode_error, "ServerHello CipherSuite not a real ciphersuite")
 
 
@@ -315,7 +318,7 @@ let client_handle_server_hello (HS #r0 r res cfg id lgref hsref) msgs =
   | C(C_HelloSent ri ch),[(ServerHello(sh),l)] ->
    (match (processServerHello cfg (!hsref).hs_ks (!hsref).hs_log ri ch (ServerHello sh,l)) with
     | Error z -> InError z
-    | Correct (n) -> 
+    | Correct (n,k) -> 
       hsref := {!hsref with
 	       hs_nego = Some n;
 	       hs_state = C(C_HelloReceived n)};
@@ -450,9 +453,68 @@ let client_handle_server_finished (HS #r0 r res cfg id lgref hsref) msgs =
        InAck)
     
 
-assume val client_handle_server_finished_13: hs -> list (hs_msg * bytes) -> ST incoming
+let processServerFinished_13 cfg n ks log msgs =
+   let rem,creq = 
+     match msgs with
+     | (EncryptedExtensions ee,_) :: (CertificateRequest cr,_) :: rem ->         
+       let _ = log @@ EncryptedExtensions(ee) in 
+       let _ = log @@ CertificateRequest(cr) in 
+       rem,true
+     | (EncryptedExtensions ee,_) :: rem ->         
+       let _ = log @@ EncryptedExtensions(ee) in 
+       rem,false in
+    match rem with
+    | [(Certificate c,_); (CertificateVerify cv,_); (Finished f,_)] 
+     when (is_Some n.n_sigAlg && (n.n_kexAlg = Kex_DHE || n.n_kexAlg = Kex_ECDHE)) -> 
+     if Cert.validate_chain c.crt_chain n.n_sigAlg cfg.peer_name cfg.ca_file then
+     let _ = log @@ Certificate(c) in
+     let lb = HandshakeLog.getHash log in
+     let cs_sigalg = Some.v n.n_sigAlg in
+     let valid = Cert.verify_signature c.crt_chain n.n_protocol_version Server None
+          cs_sigalg n.n_extensions.ne_signature_algorithms lb cv.cv_sig in
+     let _ = IO.debug_print_string("Signature validation status = "^(if valid then "OK" else "FAIL")^"\n") in
+     if true then // TODO: SIG VALIDATION CURRENTLY FAILS; this should be "if valid then"
+     let _ = log @@ CertificateVerify(cv) in
+     let lb = HandshakeLog.getHash log in
+     let svd = KeySchedule.ks_client_13_1rtt_server_finished ks lb in
+     if (equalBytes svd f.fin_vd) then 
+     	let _ = log @@ (Finished(f)) in
+	let lb = HandshakeLog.getHash log in
+	let (cvd,keys) = KeySchedule.ks_client_13_1rtt_client_finished ks lb in	
+	let cfin = {fin_vd = cvd} in
+	if creq then 
+	   let cc = {crt_chain = []} in 
+	   let ccb = log @@ Certificate(cc) in
+	   let finb = log @@ Finished(cfin) in
+	   Correct ([(Certificate(cc),ccb);(Finished(cfin),finb)],svd,keys)
+	else
+	   let finb = log @@ Finished(cfin) in
+	   Correct ([(Finished(cfin),finb)],svd,keys)
+     else Error (AD_decode_error, "Finished MAC did not verify")
+     else Error (AD_decode_error, "Certificate signature did not verify")
+     else Error (AD_decode_error, "Certificate was not valid")
+   | _ -> Error (AD_decode_error, "Unexpected state")
+
+val client_handle_server_finished_13: hs -> list (hs_msg * bytes) -> ST incoming
   (requires (fun h -> True))
   (ensures (fun h0 i h1 -> True))
+let client_handle_server_finished_13 (HS #r0 r res cfg id lgref hsref) msgs =
+  match (!hsref).hs_state with
+  | C(C_CCSReceived n vd) ->
+   (match processServerFinished_13 cfg n (!hsref).hs_ks (!hsref).hs_log msgs with
+    | Error z -> InError z
+    | Correct ([(Finished(f),fb)],svd,keys) -> 
+       hsref := {!hsref with
+                 hs_buffers = {(!hsref).hs_buffers with hs_outgoing = fb};
+  		 hs_state = C(C_Idle (Some (vd,svd)))};
+       InAck
+    | Correct ([(Certificate c,cb);(Finished f,fb)],svd,keys) -> 
+       hsref := {!hsref with
+                 hs_buffers = {(!hsref).hs_buffers with hs_outgoing = cb @| fb};
+  		 hs_state = C(C_Idle (Some (vd,svd)))};
+       InAck)
+    
+
 
 
 val server_handle_client_hello: hs -> list (hs_msg * bytes) -> ST incoming
